theories/Syntax/Expressions.v
@@ -172,6 +172,15 @@ Module Type ExpressionsOn (Import TY : Types).
   Notation "e1 < e2" := (exp_binop bop.lt e1 e2) : exp_scope.
   Notation "e1 > e2" := (exp_binop bop.gt e1 e2) : exp_scope.
   Notation "e1 <= e2" := (exp_binop bop.le e1 e2) : exp_scope.
+  Notation "e1 >= e2" := (exp_binop bop.ge e1 e2) : exp_scope.
+
+  Notation "e1 +ᵇ e2" := (exp_binop bop.bvadd e1 e2) : exp_scope.
+  Notation "e1 -ᵇ e2" := (exp_binop bop.bvadd e1 e2) : exp_scope.
+  Notation "e1 *ᵇ e2" := (exp_binop bop.bvmul e1 e2) : exp_scope.
+  Notation "e1 <ᵘ e2" := (exp_binop bop.bvult e1 e2) : exp_scope.
+  Notation "e1 >ᵘ e2" := (exp_binop bop.bvugt e1 e2) : exp_scope.
+  Notation "e1 <=ᵘ e2" := (exp_binop bop.bvule e1 e2) : exp_scope.
+  Notation "e1 >=ᵘ e2" := (exp_binop bop.bvuge e1 e2) : exp_scope.
   Notation "e1 = e2" := (exp_binop bop.eq e1 e2) : exp_scope.
   Notation "- e" := (exp_neg e) : exp_scope.
 
